prim/verif_prim.v
@@ -1,4 +1,5 @@
 Require Import VST.floyd.proofauto.
+Require Import VST.msl.iter_sepcon.
 Require Import CertiGraph.lib.List_ext.
 Require Import CertiGraph.floyd_ext.share.
 Require Import CertiGraph.graph.graph_model.
@@ -16,6 +17,59 @@ Local Open Scope Z.
 (***********************VERIFICATION***********************)
 
 (**Initialisation functions**)
+
+Lemma body_getCell: semax_body Vprog Gprog f_getCell getCell_spec.
+Proof.
+  start_function.
+  unfold undirected_matrix.
+  rewrite (SpaceAdjMatGraph_unfold' _ _ _ _ addresses u); trivial.
+  
+  assert ((Zlength (map Int.repr (Znth u (graph_to_symm_mat g)))) = SIZE). {
+    unfold graph_to_symm_mat, graph_to_mat, vert_to_list.
+    rewrite Znth_map; repeat rewrite Zlength_map.
+    all: rewrite nat_inc_list_Zlength, Z2Nat.id; lia.
+  }
+  assert (0 <= i < Zlength (map Int.repr (Znth u (graph_to_symm_mat g)))) by lia.
+  assert (0 <= i < Zlength (Znth u (graph_to_symm_mat g))). {
+    rewrite Zlength_map in H1. lia.
+  }
+
+  Intros.
+  freeze FR := (iter_sepcon _ _) (iter_sepcon _ _).
+  unfold list_rep.
+  
+  assert_PROP (force_val
+                 (sem_add_ptr_int
+                    tint
+                    Signed
+                    (force_val
+                       (sem_add_ptr_int
+                          (tarray tint SIZE)
+                          Signed
+                          (pointer_val_val graph_ptr)
+                          (Vint (Int.repr u))))
+                    (Vint (Int.repr i))) =
+               field_address
+                 (tarray tint SIZE)
+                 [ArraySubsc i]
+                 (@list_address
+                    SIZE
+                    CompSpecs
+                    (pointer_val_val graph_ptr)
+                    u)). {
+    entailer!.
+    unfold list_address. simpl.
+    rewrite field_address_offset.
+    1: { rewrite offset_offset_val; simpl; f_equal.
+         rewrite Z.add_0_l. f_equal. lia. }            
+    destruct H5 as [? [? [? [? ?]]]]. 
+    unfold field_compatible; split3; [| | split3]; simpl; auto.
+  }
+  forward. forward. 
+  thaw FR. unfold undirected_matrix.
+  rewrite (SpaceAdjMatGraph_unfold' _ _ _ _ addresses u); trivial.
+  entailer!.
+Qed.
 
 Lemma body_initialise_list: semax_body Vprog Gprog f_initialise_list initialise_list_spec.
 Proof.
@@ -146,6 +200,7 @@ rewrite <- HZlength_nat_inc_list; unfold SIZE; lia. rewrite Zlength_list_repeat;
 rewrite Zlength_list_repeat; unfold SIZE; lia.
 Qed.
 
+
 (******************PRIM'S***************)
 
 Lemma body_prim: semax_body Vprog Gprog f_prim prim_spec.
@@ -159,8 +214,9 @@ set (i:=Int.max_signed); compute in i; subst i. lia.
 repeat rewrite data_at__tarray.
 set (k:=default_val tint); compute in k; subst k.
 forward_call (Tsh, v_key, (list_repeat (Z.to_nat 8) Vundef), inf).
+1: { 
 assert_PROP (Zlength (map (fun x : Z => Vint (Int.repr x)) garbage) = SIZE). entailer!.
-forward_call (sh, (pointer_val_val parent_ptr), (map (fun x : Z => Vint (Int.repr x)) garbage), SIZE).
+forward_call (wshare_share sh, (pointer_val_val parent_ptr), (map (fun x : Z => Vint (Int.repr x)) garbage), SIZE).
 clear H garbage.
 forward_call (Tsh, v_out, (list_repeat (Z.to_nat 8) Vundef), 0).
 assert (Hrbound: 0 <= r < SIZE). apply vert_bound in Hprecon_1; auto.
@@ -596,10 +652,14 @@ break: (
   (**In queue**)
   +assert (~ In i (popped_vertices+::u)). {
     destruct (in_dec V_EqDec i (popped_vertices +:: u)). simpl in H5. inversion H5. auto.
-  }
+   }
+
+   forward_call (sh, g, gptr, (@nil val), u, i).
+
+   (*
   rewrite (graph_unfold _ _ _ u). unfold list_rep.
    2: { unfold graph_to_symm_mat, graph_to_mat.
-        rewrite Zlength_map, nat_inc_list_Zlength. rewrite Z2Nat.id. lia. unfold SIZE; lia. }
+        rewrite Zlength_map, nat_inc_list_Zlength. rewrite Z2Nat.id. lia. unfold SIZE; lia. } 
   assert_PROP (field_compatible (tarray tint SIZE) [ArraySubsc i] (offset_val (u * sizeof (tarray tint SIZE)) (pointer_val_val gptr))). entailer!.
   assert_PROP(force_val (sem_add_ptr_int tint Signed (force_val (sem_add_ptr_int (tarray tint SIZE) Signed (pointer_val_val gptr) (Vint (Int.repr u))))
    (Vint (Int.repr i))) = (field_address (tarray tint SIZE) [ArraySubsc i] (offset_val (u * sizeof (tarray tint SIZE)) (pointer_val_val gptr)))). {
@@ -615,7 +675,17 @@ break: (
     rewrite Zlength_map. rewrite Zlength_map. rewrite nat_inc_list_Zlength, Z2Nat.id; auto.
     unfold SIZE; lia. rewrite nat_inc_list_Zlength, Z2Nat.id. lia. lia.
   }
-  forward. forward.
+  2: { unfold graph_to_symm_mat.
+       rewrite graph_to_mat_Zlength; lia.
+  } *)
+
+   forward.
+   assert (1 = 1) by trivial.
+   assert (1 = 1) by trivial.
+   assert (1 = 1) by trivial.
+   (* AM: Just don't want to renumber all the hypotheses
+      going forth 
+    *)
   forward_if.
     -(*g[u][i] < ...*)
     (*implies adjacency*)
@@ -629,7 +699,8 @@ break: (
       assert (Znth i keys' <= inf). apply Hinv2_4. lia.
       (*can't lia here for some reason*) apply (Z.lt_le_trans _ (Znth i keys')); auto.
     }
-    forward. forward. forward. forward. entailer!.
+    forward. forward. forward.
+    entailer!.
     rewrite upd_Znth_same. simpl. auto. rewrite Zlength_map. rewrite HZlength_keys'. auto.
     rewrite upd_Znth_same. 2: { simpl. auto. rewrite Zlength_map. rewrite HZlength_keys'. auto. }
     forward_call (v_pq, i, Znth i (Znth u (graph_to_symm_mat g)), pq_state').
@@ -700,7 +771,6 @@ break: (
       rewrite HZlength_keys'; lia. auto.
     } (*entailer unable to solve but no change to timing*)
     time "inner loop update-because-lt-postcon (orig 71 seconds)" entailer!.
-    entailer!. (*bizarre, have to call back-to-back entailers*)
     unfold graph_to_symm_mat.
     rewrite graph_to_mat_Zlength; trivial. lia.
     -forward. (*nothing changed*)
@@ -751,8 +821,7 @@ break: (
       intros. apply Hinv2_3. lia.
     } (*entailer unable to solve but no change to timing*)
     time "inner loop no-update-because-not-lt-postcon (originally 60s)" entailer!.
-    - unfold graph_to_symm_mat.
-      rewrite graph_to_mat_Zlength; lia.
+    
   +(*nothing changed because out of pq*)
   assert (In i (popped_vertices+::u)). {
     unfold typed_false in H5. destruct (V_EqDec u i); simpl in H5. unfold Equivalence.equiv in e; subst i. apply in_or_app; right; left; auto.
@@ -1798,6 +1867,6 @@ forward.
 Exists mst fmst parents.
 (*change from popped_vertices to nat_inc_list*)
 entailer!.
-}
+
 (*Should we bother with filling a matrix for it? The original Prim doesn't bother*)
-Qed.
+Admitted
